CollapsingTowers/TwoLevelRec/OperationalSemantics/Refine.lean
@@ -1,2 +1,230 @@
 import CollapsingTowers.TwoLevelRec.OperationalSemantics.Confluence
 import CollapsingTowers.TwoLevelRec.OperationalSemantics.Congruence
+
+-- B⟦e₀⟧ ⇝ r
+-- ———————————————————————
+-- B⟦e₀⟧ ⇝ B⟦e₁⟧ ∧ e₀ ⇝ e₁
+lemma step.refine :
+  ∀ B₀ e₀ r,
+    ctx𝔹 B₀ →
+    ¬value e₀ →
+    grounded B₀⟦e₀⟧  →
+    (B₀⟦e₀⟧ ⇝ r) →
+    ∃ e₁, B₀⟦e₁⟧ = r ∧ (e₀ ⇝ e₁) :=
+  by
+  intros B₀ e₀ r HB₀ HNv HG
+  generalize HEqe : B₀⟦e₀⟧ = E₀
+  intros Hstep
+  cases Hstep
+  case pure M e₁ e₂ HM Hlc Hhead =>
+    have Hstepable := head_impl_head_stepable _ _ Hlc Hhead
+    cases HM
+    case hole =>
+      exfalso
+      apply Hstepable.HAtomic𝔹
+      apply HB₀; apply HNv
+      symm; apply HEqe
+    case cons𝔹 B₁ M HB₁ HM =>
+      have HNvM₁ := not_value.under_ctx𝕄 _ _ _ Hstepable.HNv HM
+      have ⟨HEqM, HEqB⟩ := deterministic.under_ctx𝔹 _ _ _ _ HB₀ HB₁ HEqe HNv HNvM₁
+      exists M⟦e₂⟧
+      constructor; simp [HEqB]
+      rw [HEqM]; apply step_lvl.pure
+      apply HM; apply Hlc; apply Hhead
+    case consℝ HR HM =>
+      exfalso
+      apply deterministic.under_ctx𝔹_ctxℝ
+      apply HB₀; apply HR; apply HEqe
+      apply HNv; apply not_value.under_ctx𝕄
+      apply Hstepable.HNv; apply HM
+  case reflect M E _ HP HE _ =>
+    rw [HEqe] at HG
+    have HM := rewrite.ctxℙ_ctx𝕄 _ _ HP
+    have HG := grounded.decompose_ctx𝕄 _ _ _ HM HG
+    have HG := grounded.decompose_ctx𝔼 _ _ HE HG
+    simp at HG
+
+-- B⟦e⟧ ⇝ₖ v
+-- —————————————————————————————————
+-- k = i + j ∧ e ⇝ᵢ v𝕖 ∧ B⟦v𝕖⟧ ⇝ⱼ v
+lemma stepn_indexed.refine :
+  ∀ B e₀ v k,
+    ctx𝔹 B →
+    value v →
+    grounded B⟦e₀⟧  →
+    (B⟦e₀⟧ ⇝ ⟦k⟧ v) →
+    ∃ i j v𝕖,
+      i + j = k ∧
+      value v𝕖 ∧
+      (e₀ ⇝ ⟦i⟧ v𝕖) ∧
+      (B⟦v𝕖⟧ ⇝ ⟦j⟧ v) :=
+  by
+  intros B e₀ v k HB
+  generalize HEqe₀ : B⟦e₀⟧ = E
+  intros Hvalue HG₀ Hstep
+  induction Hstep generalizing e₀
+  case refl =>
+    exfalso; apply not_value.under_ctx𝔹
+    apply HB; rw [HEqe₀]; apply Hvalue
+  case multi k im₀ im₁ im₂ Hstep Hstepn IH =>
+    rw [← HEqe₀] at Hstep
+    match value.decidable e₀ with
+    | isTrue Hvalue =>
+      exists 0, k + 1, e₀
+      constructor; omega
+      constructor; apply Hvalue
+      constructor; apply stepn_indexed.refl
+      apply stepn_indexed.multi; apply Hstep; apply Hstepn
+    | isFalse HNv =>
+      rw [← HEqe₀] at HG₀
+      have ⟨e₁, HEqe₁, Hstep₀⟩ := step.refine _ _ _ HB HNv HG₀ Hstep
+      have HG₁ := grounded.under_step _ _ Hstep HG₀
+      have ⟨i, j, v𝕖, HEqk, Hvalue, Hstep₁, Hstep₂⟩ := IH _ HEqe₁ Hvalue HG₁
+      exists i + 1, j, v𝕖
+      constructor; omega
+      constructor; apply Hvalue
+      constructor; apply stepn_indexed.multi
+      apply Hstep₀; apply Hstep₁; apply Hstep₂
+
+lemma stepn_indexed.refine.lam :
+  ∀ e arg v j,
+    value (.lam e) → value arg → value v →
+    ((.app₁ (.lam e) arg) ⇝ ⟦j⟧ v) →
+    ∃ i,
+      i + 1 = j ∧
+      ((opening 0 arg e) ⇝ ⟦i⟧ v) :=
+  by
+  intros e arg v j HvalueFun HvalueArg Hvalue Hstep
+  have HstepHead : (.app₁ (.lam e) arg) ⇝ ⟦1⟧ (opening 0 arg e) :=
+    by
+    apply stepn_indexed.multi _ _ _ _ _ (stepn_indexed.refl _)
+    apply step_lvl.pure id; apply ctx𝕄.hole
+    constructor; apply lc.value; apply HvalueFun; apply lc.value; apply HvalueArg
+    apply head.app₁; apply HvalueArg
+  have ⟨z, i, r, HEqIndex, Hstepl, Hstepr⟩ := stepn_indexed.church_rosser _ _ _ _ _ Hstep HstepHead
+  have ⟨HEqv, Hz⟩ := stepn_indexed.value_impl_termination _ _ _ Hvalue Hstepl
+  exists i
+  constructor; omega
+  rw [HEqv]; apply Hstepr
+
+lemma stepn_indexed.refine.app₁ :
+  ∀ f arg v j,
+    value v →
+    grounded (.app₁ f arg) →
+    ((.app₁ f arg) ⇝ ⟦j⟧ v) →
+    ∃ i₀ i₁ i₂ fᵥ argᵥ,
+      i₀ + i₁ + i₂ = j ∧
+      value fᵥ ∧ value argᵥ ∧
+      (f ⇝ ⟦i₀⟧ fᵥ) ∧ (arg ⇝ ⟦i₁⟧ argᵥ) ∧ ((.app₁ fᵥ argᵥ) ⇝ ⟦i₂⟧ v) :=
+  by
+  intros f arg v j Hvalue HG₀ Hstep
+  have ⟨HGFun, HGArg⟩ := HG₀
+  have Hlc := lc.under_stepn_indexed _ _ _ Hstep (lc.value _ Hvalue)
+  have ⟨i₀, k, fᵥ, HEqj, HvalueFun, Hstep₀, Hstep⟩ := stepn_indexed.refine _ _ _ _ (ctx𝔹.appl₁ _ Hlc.right) Hvalue HG₀ Hstep
+  have HGFunᵥ := grounded.under_stepn _ _ (stepn_indexed_impl_stepn _ _ _ Hstep₀) HGFun
+  have HG₁ : grounded (.app₁ fᵥ arg) := by constructor; apply HGFunᵥ; apply HGArg
+  have ⟨i₁, i₂, argᵥ, HEqj, HvalueArg, Hstep₁, Hstep₂⟩ := stepn_indexed.refine _ _ _ _ (ctx𝔹.appr₁ _ HvalueFun) Hvalue HG₁ Hstep
+  exists i₀, i₁, i₂, fᵥ, argᵥ
+  constructor; omega
+  constructor; apply HvalueFun
+  constructor; apply HvalueArg
+  constructor; apply Hstep₀
+  constructor; apply Hstep₁
+  apply Hstep₂
+
+lemma stepn_indexed.refine.lets :
+  ∀ b e v j,
+    value v →
+    grounded (.lets b e) →
+    ((.lets b e) ⇝ ⟦j⟧ v) →
+    ∃ i₀ i₁ bᵥ,
+      i₀ + 1 + i₁ = j ∧
+      value bᵥ ∧
+      (b ⇝ ⟦i₀⟧ bᵥ) ∧ ((opening 0 bᵥ e) ⇝ ⟦i₁⟧ v) :=
+  by
+  intros b e v j Hvalue HG Hstep
+  have Hlc := lc.under_stepn_indexed _ _ _ Hstep (lc.value _ Hvalue)
+  have ⟨i₀, k, bᵥ, HEqj, HvalueBind, Hstep₀, Hstep⟩ := stepn_indexed.refine _ _ _ _ (ctx𝔹.lets _ Hlc.right) Hvalue HG Hstep
+  have HstepHead : (.lets bᵥ e) ⇝ ⟦1⟧ (opening 0 bᵥ e) :=
+    by
+    apply stepn_indexed.multi _ _ _ _ _ (stepn_indexed.refl _)
+    apply step_lvl.pure id; apply ctx𝕄.hole
+    constructor; apply lc.value; apply HvalueBind; apply Hlc.right
+    apply head.lets; apply HvalueBind
+  have ⟨z, i₁, r, HEqIndex, Hstepl, Hstepr⟩ := stepn_indexed.church_rosser _ _ _ _ _ Hstep HstepHead
+  have ⟨HEqv, Hz⟩ := stepn_indexed.value_impl_termination _ _ _ Hvalue Hstepl
+  exists i₀, i₁, bᵥ
+  constructor; omega
+  constructor; apply HvalueBind
+  constructor; apply Hstep₀
+  rw [HEqv]; apply Hstepr
+
+lemma stepn_indexed.refine.fix₁ :
+  ∀ f v j,
+    value v →
+    grounded (.fix₁ f) →
+    ((.fix₁ f) ⇝ ⟦j⟧ v) →
+    ∃ i fᵥ,
+      i + 1 = j ∧
+      value fᵥ ∧
+      (f ⇝ ⟦i⟧ fᵥ) ∧ v = .lam (.app₁ (.app₁ fᵥ (.fix₁ fᵥ)) (.bvar 0))  :=
+  by
+  intros f v j Hvalue₀ HG Hstep
+  have ⟨i₀, k, fᵥ, HEqj, HvalueFun, Hstep₀, Hstep⟩ := stepn_indexed.refine _ _ _ _ ctx𝔹.fix₁ Hvalue₀ HG Hstep
+  have HstepHead : (.fix₁ fᵥ) ⇝ ⟦1⟧ .lam (.app₁ (.app₁ fᵥ (.fix₁ fᵥ)) (.bvar 0)) :=
+    by
+    apply stepn_indexed.multi _ _ _ _ _ (stepn_indexed.refl _)
+    apply step_lvl.pure id; apply ctx𝕄.hole
+    simp; apply lc.value; apply HvalueFun
+    apply head.fix₁; apply HvalueFun
+  have Hvalue₁ : value (.lam (.app₁ (.app₁ fᵥ (.fix₁ fᵥ)) (.bvar 0))) :=
+    by
+    apply value.lam; simp; apply lc.inc
+    apply lc.value; apply HvalueFun; omega
+  have ⟨z₀, z₁, r, HEqIndex, Hstepl, Hstepr⟩ := stepn_indexed.church_rosser _ _ _ _ _ Hstep HstepHead
+  have ⟨HEqv₀, Hz₀⟩ := stepn_indexed.value_impl_termination _ _ _ Hvalue₀ Hstepl
+  have ⟨HEqv₁, Hz₁⟩ := stepn_indexed.value_impl_termination _ _ _ Hvalue₁ Hstepr
+  exists i₀, fᵥ
+  constructor; omega
+  constructor; apply HvalueFun
+  constructor; apply Hstep₀
+  rw [HEqv₀, HEqv₁]
+
+lemma stepn_indexed.refine.fix₁.induction :
+  ∀ f arg v j,
+    value f → value arg → value v →
+    grounded (.fix₁ f) →
+    ((.app₁ (.lam (.app₁ (.app₁ f (.fix₁ f)) (.bvar 0))) arg) ⇝ ⟦j⟧ v) →
+    ∃ i,
+      i + 2 = j ∧
+      (.app₁ (.app₁ f (.lam (.app₁ (.app₁ f (.fix₁ f)) (.bvar 0)))) arg) ⇝ ⟦i⟧ v :=
+  by
+  intros f arg v j HvalueFun HvalueArg Hvalue HG Hstep
+  have HstepHead₀ : (.app₁ (.lam (.app₁ (.app₁ f (.fix₁ f)) (.bvar 0))) arg) ⇝ (.app₁ (.app₁ f (.fix₁ f)) arg) :=
+    by
+    apply step_lvl.pure id; apply ctx𝕄.hole
+    simp; constructor
+    apply lc.inc; apply lc.value; apply HvalueFun; omega
+    apply lc.value; apply HvalueArg
+    have HEqSubst₀ : .app₁ (.app₁ f (.fix₁ f)) arg = opening 0 arg (.app₁ (.app₁ f (.fix₁ f)) (.bvar 0)) :=
+      by
+      simp; rw [identity.opening]
+      apply lc.inc; apply lc.value; apply HvalueFun; omega
+    rw [HEqSubst₀]; apply head.app₁; apply HvalueArg
+  have HstepHead₁ : (.app₁ (.app₁ f (.fix₁ f)) arg) ⇝ (.app₁ (.app₁ f (.lam (.app₁ (.app₁ f (.fix₁ f)) (.bvar 0)))) arg) :=
+    by
+    apply step.grounded.congruence_under_ctx𝔹 _ _ _ (ctx𝔹.appl₁ _ (lc.value _ HvalueArg)) (by simp; apply HG)
+    apply step.grounded.congruence_under_ctx𝔹 _ _ _ (ctx𝔹.appr₁ _ HvalueFun) (by simp; apply HG)
+    apply step_lvl.pure id; apply ctx𝕄.hole
+    simp; apply lc.value; apply HvalueFun
+    apply head.fix₁; apply HvalueFun
+  have HstepHead : (.app₁ (.lam (.app₁ (.app₁ f (.fix₁ f)) (.bvar 0))) arg) ⇝ ⟦2⟧ (.app₁ (.app₁ f (.lam (.app₁ (.app₁ f (.fix₁ f)) (.bvar 0)))) arg) :=
+    by
+    apply stepn_indexed.multi; apply HstepHead₀
+    apply stepn_indexed.multi; apply HstepHead₁
+    apply stepn_indexed.refl
+  have ⟨z, i, r, HEqIndex, Hstepl, Hstepr⟩ := stepn_indexed.church_rosser _ _ _ _ _ Hstep HstepHead
+  have ⟨HEqv, Hz⟩ := stepn_indexed.value_impl_termination _ _ _ Hvalue Hstepl
+  exists i
+  constructor; omega
+  rw [HEqv]; apply Hstepr
